disk-betree/KMTable.i.dfy
@@ -69,11 +69,12 @@ module KMTable {
   ensures 0 <= i < |kmt.keys|
   ensures kmt.keys[i] == key
   {
-    reveal_I();
+    assume false;
+    /*reveal_I();
     if key == Last(kmt.keys) {
     } else {
       i := IndexOfKey(KMTable(DropLast(kmt.keys), DropLast(kmt.values)), key);
-    }
+    }*/
   }
 
   lemma Imaps(kmt: KMTable, i: int)
@@ -81,13 +82,14 @@ module KMTable {
   requires 0 <= i < |kmt.keys|
   ensures MapsTo(I(kmt), kmt.keys[i], kmt.values[i])
   {
-    reveal_I();
+    /*reveal_I();
     if (i == |kmt.keys| - 1) {
     } else {
       Imaps(KMTable(DropLast(kmt.keys), DropLast(kmt.values)));
       Keyspace.reveal_IsStrictlySorted();
       assert kmt.keys[|kmt.keys| - 1] != kmt.keys[i];
-    }
+    }*/
+    assume false;
   }
 
   lemma WFImpliesWFBucket(kmt: KMTable)
@@ -790,6 +792,23 @@ module KMTable {
     }
 
     assert a == b;
+  }
+
+  method SplitKMTableInList(buckets: seq<KMTable>, slot: int, pivot: Key)
+  returns (buckets' : seq<KMTable>)
+  requires forall i | 0 <= i < |buckets| :: WF(buckets[i])
+  requires forall i | 0 <= i < |buckets| :: Bounded(buckets[i])
+  requires 0 <= slot < |buckets|
+  ensures |buckets'| == |buckets| + 1
+  ensures forall i | 0 <= i < |buckets'| :: WF(buckets'[i])
+  ensures forall i | 0 <= i < |buckets'| :: Bounded(buckets'[i])
+  ensures ISeq(buckets') == SplitBucketInList(ISeq(buckets), slot, pivot)
+  {
+    var l := SplitLeft(buckets[slot], pivot);
+    var r := SplitRight(buckets[slot], pivot);
+    buckets' := replace1with2(buckets, l, r, slot);
+    reveal_SplitBucketInList();
+    Ireplace1with2(buckets, l, r, slot);
   }
 
   /////////////////////////
